Add proofs for eBPF-backend

cparser/Machine.ml
@@ -247,7 +247,7 @@ let aarch64_apple =
   { aarch64 with char_signed = true }
 
 let ebpf =
-  { ilp32ll64 with name = "ebpf" } (* TODO *)
+  { ilp32ll64 with name = "ebpf" }
 
 (* Add GCC extensions re: sizeof and alignof *)
 
