ebpf/Asmgenproof1.v
@@ -1,0 +1,430 @@
+(* *********************************************************************)
+(*                                                                     *)
+(*              The Compcert verified compiler                         *)
+(*                                                                     *)
+(*          Xavier Leroy, INRIA Paris-Rocquencourt                     *)
+(*                                                                     *)
+(*  Copyright Institut National de Recherche en Informatique et en     *)
+(*  Automatique.  All rights reserved.  This file is distributed       *)
+(*  under the terms of the INRIA Non-Commercial License Agreement.     *)
+(*                                                                     *)
+(* *********************************************************************)
+
+Require Import Coqlib Errors Maps.
+Require Import AST Zbits Integers Floats Values Memory Globalenvs.
+Require Import Op Locations Mach Conventions.
+Require Import Asm Asmgen Asmgenproof0.
+
+(** Properties of registers *)
+
+Lemma ireg_of_not_R10:
+  forall m r, ireg_of m = OK r -> IR r <> IR R10.
+Proof.
+  intros. erewrite <- ireg_of_eq; eauto with asmgen.
+Qed.
+
+Lemma ireg_of_not_R10':
+  forall m r, ireg_of m = OK r -> r <> R10.
+Proof.
+  intros. apply ireg_of_not_R10 in H. congruence.
+Qed.
+
+Global Hint Resolve ireg_of_not_R10 ireg_of_not_R10': asmgen.
+
+(** Useful simplification tactic *)
+
+Ltac Simplif :=
+  ((rewrite nextinstr_inv by eauto with asmgen)
+  || (rewrite nextinstr_inv1 by eauto with asmgen)
+  || (rewrite Pregmap.gss)
+  || (rewrite nextinstr_pc)
+  || (rewrite Pregmap.gso by eauto with asmgen)); auto with asmgen.
+
+Ltac Simpl := repeat Simplif.
+
+(** * Correctness of eBPF constructor functions *)
+
+Section CONSTRUCTORS.
+
+Variable ge: genv.
+Variable fn: function.
+
+(** Add offset to pointer *)
+
+Lemma addptrofs_correct:
+  forall rd r1 n k rs m,
+  exists rs',
+     exec_straight ge fn (addptrofs rd r1 n k) rs m k rs' m
+  /\ Val.lessdef (Val.offset_ptr rs#r1 n) rs'#rd
+  /\ forall r, r <> PC -> r <> rd -> rs'#r = rs#r.
+Proof.
+  unfold addptrofs; intros.
+  destruct (Ptrofs.eq_dec n Ptrofs.zero).
+  - subst n. econstructor; split.
+    apply exec_straight_one. simpl; constructor. auto.
+    split. Simpl. simpl. destruct (rs r1); simpl; auto. rewrite Ptrofs.add_zero; auto.
+    intros; Simpl.
+  - eexists; split.
+    eapply exec_straight_two; reflexivity.
+    split; intros; Simpl.
+    simpl.
+    unfold Val.add, Val.offset_ptr.
+    destruct (rs r1); try constructor.
+    change Archi.ptr64 with false; simpl.
+    apply Val.lessdef_same; f_equal; f_equal.
+    rewrite Ptrofs.of_int_to_int by auto.
+    reflexivity.
+Qed.
+
+(** Translation of conditional branches *)
+
+Lemma transl_cbranch_signed_correct:
+  forall cmp r1 r2 lbl (rs: regset) m b,
+  Val.cmp_bool cmp rs#(IR r1) (eval_reg_imm rs r2) = Some b ->
+  exec_instr ge fn (transl_cbranch_signed cmp r1 r2 lbl) rs m =
+  exec_branch fn lbl rs m (Some b).
+Proof.
+  intros. destruct cmp; simpl; rewrite ? H; try reflexivity.
+  - destruct rs#r1; simpl in H; try discriminate.
+    destruct (eval_reg_imm rs r2); simpl in H; try discriminate.
+    inv H; simpl.
+    reflexivity.
+  - destruct rs#r1; simpl in H; try discriminate.
+    destruct (eval_reg_imm rs r2); simpl in H; try discriminate.
+    inv H; simpl.
+    reflexivity.
+Qed.
+
+Lemma transl_cbranch_unsigned_correct:
+  forall cmp r1 r2 lbl (rs: regset) m b,
+  Val.cmpu_bool (Mem.valid_pointer m) cmp rs#(IR r1) (eval_reg_imm rs r2) = Some b ->
+  exec_instr ge fn (transl_cbranch_unsigned cmp r1 r2 lbl) rs m =
+  exec_branch fn lbl rs m (Some b).
+Proof.
+  intros. destruct cmp; simpl; rewrite ? H; reflexivity.
+Qed.
+
+Ltac ArgsInv :=
+  repeat (match goal with
+  | [ H: Error _ = OK _ |- _ ] => discriminate
+  | [ H: match ?args with nil => _ | _ :: _ => _ end = OK _ |- _ ] => destruct args
+  | [ H: bind _ _ = OK _ |- _ ] => monadInv H
+  | [ H: match _ with left _ => _ | right _ => assertion_failed end = OK _ |- _ ] => monadInv H; ArgsInv
+  | [ H: match _ with true => _ | false => assertion_failed end = OK _ |- _ ] => monadInv H; ArgsInv
+  end);
+  subst;
+  repeat (match goal with
+  | [ H: ireg_of _ = OK _ |- _ ] => simpl in *; rewrite (ireg_of_eq _ _ H) in *
+  | [ H: freg_of _ = OK _ |- _ ] => simpl in *; rewrite (freg_of_eq _ _ H) in *
+  end).
+
+Lemma transl_cbranch_correct_1:
+  forall cond args lbl k c m ms b sp rs m',
+  transl_cbranch cond args lbl k = OK c ->
+  eval_condition cond (List.map ms args) m = Some b ->
+  agree ms sp rs ->
+  Mem.extends m m' ->
+  exists rs', exists insn,
+     exec_straight_opt ge fn c rs m' (insn :: k) rs' m'
+  /\ exec_instr ge fn insn rs' m' = exec_branch fn lbl rs' m' (Some b)
+  /\ forall r, r <> PC -> rs'#r = rs#r.
+Proof.
+  intros until m'; intros TRANSL EVAL AG MEXT.
+  set (vl' := map rs (map preg_of args)).
+  assert (EVAL': eval_condition cond vl' m' = Some b).
+  { apply eval_condition_lessdef with (map ms args) m; auto. eapply preg_vals; eauto. }
+  clear EVAL MEXT AG.
+  destruct cond; simpl in TRANSL; ArgsInv.
+  - exists rs, (transl_cbranch_signed c0 x (inl x0) lbl).
+    intuition auto. constructor. apply transl_cbranch_signed_correct; auto.
+  - exists rs, (transl_cbranch_unsigned c0 x (inl x0) lbl).
+    intuition auto. constructor. apply transl_cbranch_unsigned_correct; auto.
+  - exists rs, (transl_cbranch_signed c0 x (inr n) lbl).
+    intuition auto. constructor. apply transl_cbranch_signed_correct; auto.
+  - exists rs, (transl_cbranch_unsigned c0 x (inr n) lbl).
+    intuition auto. constructor. apply transl_cbranch_unsigned_correct; auto.
+Qed.
+
+Lemma transl_cbranch_correct_true:
+  forall cond args lbl k c m ms sp rs m',
+  transl_cbranch cond args lbl k = OK c ->
+  eval_condition cond (List.map ms args) m = Some true ->
+  agree ms sp rs ->
+  Mem.extends m m' ->
+  exists rs', exists insn,
+     exec_straight_opt ge fn c rs m' (insn :: k) rs' m'
+  /\ exec_instr ge fn insn rs' m' = goto_label fn lbl rs' m'
+  /\ forall r, r <> PC -> rs'#r = rs#r.
+Proof.
+  intros. eapply transl_cbranch_correct_1 with (b := true); eauto.
+Qed.
+
+Lemma transl_cbranch_correct_false:
+  forall cond args lbl k c m ms sp rs m',
+  transl_cbranch cond args lbl k = OK c ->
+  eval_condition cond (List.map ms args) m = Some false ->
+  agree ms sp rs ->
+  Mem.extends m m' ->
+  exists rs',
+     exec_straight ge fn c rs m' k rs' m'
+  /\ forall r, r <> PC -> rs'#r = rs#r.
+Proof.
+  intros. exploit transl_cbranch_correct_1; eauto. simpl.
+  intros (rs' & insn & A & B & C).
+  exists (nextinstr rs').
+  split. eapply exec_straight_opt_right; eauto. apply exec_straight_one; auto.
+  intros; Simpl.
+Qed.
+
+
+(** Translation of condition operators *)
+
+Ltac TranslCondSimpl :=
+  econstructor; split;
+  [ apply exec_straight_one; [ simpl; eauto; try reflexivity | reflexivity ]
+  | split; intros; Simpl ].
+
+Lemma transl_cond_signed_correct:
+  forall cmp r1 r2 k rs m,
+  exists rs',
+     exec_straight ge fn (transl_cond_signed cmp r1 r2 :: k) rs m k rs' m
+  /\ Val.lessdef (Val.cmp cmp rs#r1 (eval_reg_imm rs r2)) rs'#r1
+  /\ forall r, r <> PC -> r <> r1 -> rs'#r = rs#r.
+Proof.
+  intros. destruct cmp; simpl; TranslCondSimpl.
+  unfold eval_cmp; destruct (rs#r1); auto; destruct (eval_reg_imm rs r2); auto.
+  unfold eval_cmp; destruct (rs#r1); auto; destruct (eval_reg_imm rs r2); auto.
+Qed.
+
+Lemma transl_cond_unsigned_correct:
+  forall cmp r1 r2 k rs m,
+  exists rs',
+     exec_straight ge fn (transl_cond_unsigned cmp r1 r2 :: k) rs m k rs' m
+  /\ Val.lessdef (Val.cmpu (Mem.valid_pointer m) cmp rs#r1 (eval_reg_imm rs r2)) rs'#r1
+  /\ forall r, r <> PC -> r <> r1 -> rs'#r = rs#r.
+Proof.
+  intros. destruct cmp; simpl; TranslCondSimpl.
+Qed.
+
+Lemma transl_cond_op_correct:
+  forall cond rd args k c rs m,
+  transl_cond_op cond rd args k = OK c ->
+  exists rs',
+     exec_straight ge fn c rs m k rs' m
+  /\ Val.lessdef (Val.of_optbool (eval_condition cond (map rs (map preg_of args)) m)) rs'#(preg_of rd)
+  /\ forall r, r <> PC -> r <> (preg_of rd) -> rs'#r = rs#r.
+Proof.
+  assert (MKTOT: forall ob, Val.of_optbool ob = Val.maketotal (option_map Val.of_bool ob)).
+  { destruct ob as [[]|]; reflexivity. }
+  intros until m; intros TR.
+  destruct cond; simpl in TR; ArgsInv.
+  - (* cmp *)
+    exploit transl_cond_signed_correct; eauto.
+    intros (rs' & A & B & C). exists rs'; eauto.
+  - (* cmpu *)
+    exploit transl_cond_unsigned_correct; eauto.
+    intros (rs' & A & B & C). exists rs'; eauto.
+  - (* cmpimm *)
+    exploit transl_cond_signed_correct; eauto.
+    intros (rs' & A & B & C). exists rs'; eauto.
+  - (* cmpuimm *)
+    exploit transl_cond_unsigned_correct; eauto.
+    intros (rs' & A & B & C). exists rs'; eauto.
+Qed.
+
+
+(* Translation of arithmetic operations *)
+
+Ltac SimplEval H :=
+  match type of H with
+  | Some _ = None _ => discriminate
+  | Some _ = Some _ => inv H
+  | ?a = Some ?b => let A := fresh in assert (A: Val.maketotal a = b) by (rewrite H; reflexivity)
+end.
+
+Ltac TranslOpSimpl :=
+  econstructor; split;
+  [ apply exec_straight_one; [ simpl; eauto; try reflexivity | reflexivity ]
+  | split; [ apply Val.lessdef_same; Simpl; fail | intros; Simpl; fail ] ].
+
+Ltac TranslALUOpSimpl EV :=
+  econstructor; split;
+  [ apply exec_straight_one; [ unfold exec_instr, exec_alu; simpl; rewrite EV; try reflexivity | reflexivity]
+  | split; [ apply Val.lessdef_same; Simpl; fail | intros; Simpl; fail ] ].
+
+
+Lemma transl_op_correct:
+  forall op args res k (rs: regset) m v c,
+  transl_op op args res k = OK c ->
+  eval_operation ge (rs#SP) op (map rs (map preg_of args)) m = Some v ->
+  exists rs',
+     exec_straight ge fn c rs m k rs' m
+  /\ Val.lessdef v rs'#(preg_of res)
+  /\ forall r, data_preg r = true -> r <> preg_of res -> preg_notin r (destroyed_by_op op) -> rs' r = rs r.
+Proof.
+  assert (SAME: forall v1 v2, v1 = v2 -> Val.lessdef v2 v1). { intros; subst; auto. }
+Opaque Int.eq.
+  intros until c; intros TR EV.
+  unfold transl_op in TR; destruct op; ArgsInv; simpl in EV; SimplEval EV; try TranslOpSimpl.
+
+- (* addrstack *)
+  exploit addptrofs_correct; intros (rs' & A & B & C).
+  exists rs'; split; [ exact A | auto with asmgen ].
+
+- (* neg *)
+  econstructor; split.
+  apply exec_straight_one; reflexivity.
+  split.
+  + apply Val.lessdef_same; Simpl.
+    unfold Val.neg, Val.mul, eval_reg_imm.
+    destruct (rs x); try reflexivity.
+    f_equal; symmetry; apply Int.mul_mone.
+  + intros; Simpl.
+
+  (* divu, divuimm, modu, moduimm *)
+- TranslALUOpSimpl EV.
+- TranslALUOpSimpl EV.
+- TranslALUOpSimpl EV.
+- TranslALUOpSimpl EV.
+
+- (* cond *)
+  exploit transl_cond_op_correct; eauto. intros (rs' & A & B & C).
+  exists rs'; split. eexact A. eauto with asmgen.
+Qed.
+
+Lemma stack_load_correct:
+  forall ofs ty dst k c (rs: regset) m v,
+  stack_load ofs ty dst k = OK c ->
+  Mem.loadv (chunk_of_type ty) m (Val.offset_ptr rs#SP ofs) = Some v ->
+  exists rs',
+     exec_straight ge fn c rs m k rs' m
+  /\ rs'#(preg_of dst) = v
+  /\ forall r, r <> PC -> r <> preg_of dst -> rs'#r = rs#r.
+Proof.
+  intros until v. intros LOAD TR.
+  unfold stack_load in LOAD; ArgsInv.
+  econstructor. split.
+  - apply exec_straight_one. simpl; unfold exec_load.
+    + assert (H: Mem.loadv (size_to_memory_chunk x0) m (Val.offset_ptr (rs R10) ofs) = Some v). {
+        unfold chunk_of_type in TR.
+        unfold size_to_memory_chunk.
+        destruct ty, x0; try discriminate; auto.
+      }
+      rewrite H.
+      reflexivity.
+    + Simpl.
+  - split; intros; Simpl.
+Qed.
+
+Lemma stack_store_correct:
+  forall ofs ty src k c (rs: regset) m m',
+  stack_store ofs ty src k = OK c ->
+  Mem.storev (chunk_of_type ty) m (Val.offset_ptr rs#SP ofs) rs#(preg_of src) = Some m' ->
+  exists rs',
+     exec_straight ge fn c rs m k rs' m'
+  /\ forall r, r <> PC -> rs'#r = rs#r.
+Proof.
+  intros until m'. intros STORE TR.
+  unfold stack_store in STORE; ArgsInv.
+  econstructor. split.
+  - apply exec_straight_one. simpl; unfold exec_store.
+    + assert (H: Mem.storev (size_to_memory_chunk x0) m (Val.offset_ptr (rs R10) ofs) (rs x) = Some m'). {
+        unfold chunk_of_type in TR.
+        unfold size_to_memory_chunk.
+        destruct ty, x0; try discriminate; auto.
+      }
+      simpl.
+      rewrite H.
+      reflexivity.
+    + Simpl.
+  - intros; Simpl.
+Qed.
+
+Lemma transl_load_common_correct:
+  forall chunk k i op (x x0: ireg) (rs: regset) m a v,
+  Val.offset_ptr (rs x0) i = a ->
+  Mem.loadv chunk m a = Some v ->
+  transl_memory_access chunk = OK op ->
+  exists rs',
+     exec_straight ge fn (Pload op x x0 i :: k) rs m k rs' m
+  /\ rs'#x = v
+  /\ forall r, r <> PC -> r <> x -> rs'#r = rs#r.
+Proof.
+  intros until v. intros EV LOAD TR.
+  econstructor. split.
+  - apply exec_straight_one; simpl; unfold exec_load.
+    + assert (H: Mem.loadv (size_to_memory_chunk op) m a = Some v). {
+        unfold transl_memory_access in TR.
+        destruct chunk, op; try discriminate; auto.
+      }
+      rewrite EV, H.
+      reflexivity.
+    + Simpl.
+  - split; intros; Simpl.
+Qed.
+
+Lemma transl_load_correct:
+  forall chunk addr args dst k c (rs: regset) m a v,
+  transl_load chunk addr args dst k = OK c ->
+  eval_addressing ge rs#SP addr (map rs (map preg_of args)) = Some a ->
+  Mem.loadv chunk m a = Some v ->
+  exists rs',
+     exec_straight ge fn c rs m k rs' m
+  /\ rs'#(preg_of dst) = v
+  /\ forall r, r <> PC -> r <> preg_of dst -> rs'#r = rs#r.
+Proof.
+  intros until v; intros TR EV LOAD.
+  destruct addr, args; simpl in TR; ArgsInv.
+  - unfold transl_memory_access in EQ0.
+    inversion EV.
+    destruct chunk; try discriminate; eapply transl_load_common_correct; eauto.
+
+  - unfold transl_memory_access in EQ1.
+    inversion EV.
+    destruct chunk; try discriminate; eapply transl_load_common_correct; eauto.
+Qed.
+
+Lemma transl_store_common_correct:
+  forall chunk k i op (x x0: ireg) (rs: regset) m m' a,
+  Val.offset_ptr (rs x0) i = a ->
+  Mem.storev chunk m a (rs x) = Some m' ->
+  transl_memory_access chunk = OK op ->
+  exists rs',
+     exec_straight ge fn (Pstore op x0 (inl x) i :: k) rs m k rs' m'
+  /\ forall r, r <> PC -> rs'#r = rs#r.
+Proof.
+  intros until a. intros EV STORE TR.
+  econstructor. split.
+  - apply exec_straight_one; simpl; unfold exec_store.
+    + assert (H: Mem.storev (size_to_memory_chunk op) m a (rs x) = Some m'). {
+        unfold transl_memory_access in TR.
+        destruct chunk, op; try discriminate; auto.
+      }
+      simpl.
+      rewrite EV, H.
+      reflexivity.
+    + Simpl.
+  - intros; Simpl.
+Qed.
+
+Lemma transl_store_correct:
+  forall chunk addr args src k c (rs: regset) m a m',
+  transl_store chunk addr args src k = OK c ->
+  eval_addressing ge rs#SP addr (map rs (map preg_of args)) = Some a ->
+  Mem.storev chunk m a rs#(preg_of src) = Some m' ->
+  exists rs',
+     exec_straight ge fn c rs m k rs' m'
+  /\ forall r, r <> PC -> rs'#r = rs#r.
+Proof.
+  intros until m'; intros TR EV STORE.
+  destruct addr, args; simpl in TR; ArgsInv.
+  - unfold transl_memory_access in EQ0.
+    inversion EV.
+    destruct chunk; try discriminate; eapply transl_store_common_correct; eauto.
+
+  - unfold transl_memory_access in EQ1.
+    inversion EV.
+    destruct chunk; try discriminate; eapply transl_store_common_correct; eauto.
+Qed.
+
+End CONSTRUCTORS.
